\documentclass[12pt]{article}

\usepackage{amsmath, amssymb, xypic}
\usepackage[margin=1in]{geometry}

\newcommand{\norm}[1]{\left\lVert#1\right\rVert}

\begin{document}
\noindent \textbf{Name:} 

\begin{center}
Warm-up \#11
\end{center}

\noindent Let $f : X \to Y$ be a function. For a subset $V \subset Y$, let $f^{-1}(V)$ denote the preimage of $V$ defined by 
\[
f^{-1}(V) = \{x \in X : f(x) \in V\}.
\]
\begin{enumerate}
\item[(a)] Show that $f(f^{-1}(V)) \subset V$. If $f$ is surjective, show that $f(f^{-1}(V)) = V$. 
\item[(b)] For a subset $U \subset X$, show that $U \subset f^{-1}(f(U))$. If $f$ is injective, show that $U = f^{-1}(f(U)).$
\end{enumerate}
\end{document}